theories/Interp/HandlerFacts.v
@@ -28,11 +28,11 @@ Open Scope itree_scope.
 Lemma eh_cmp_id_left_strong {A R} (t : itree A R)
   : interp (id_ A) t ≈ t.
 Proof.
-  revert t. wstep. wcofix CIH. intros.
+  revert t. gstep. gcofix CIH. intros.
   rewrite unfold_interp. rewrite (itree_eta t) at 2.
-  destruct (observe t); simpl; try (wstep; constructor; eauto with paco; fail).
+  destruct (observe t); simpl; try (gstep; constructor; eauto with paco; fail).
   unfold id_, Id_Handler, Handler.id_, ITree.send. rewrite bind_vis_.
-  wstep. do 2 constructor.
+  gstep. do 2 constructor.
   right; rewrite bind_ret; auto with paco.
 Qed.
 
